src/tls/Extract0.fst
@@ -100,7 +100,7 @@ let create_psk #d #u i a =
   lemma_corrupt_invariant i "" Extract;
   if flag_KEF0 d && honest' then
     let t' = secret d u i' in
-    let r: mref_secret d u i' = MR.m_alloc #(option t') #(ssa #t') there None in
+    let r: mref_secret d u i' = ralloc #(option t') #(ssa #t') there None in
     (| (), ideal_psk #d #u #i' r |)
   else
     (| (), real_psk #d #u #i' (sample (secret_len a)) |)
@@ -150,17 +150,17 @@ let extract0 #d #u #i k a =
   if flag_KEF0 d && honest'
   then
     let k: mref_secret d u i' = psk_ideal p in
-    match MR.m_read k with
+    match !k with
     | Some extract -> extract
     | None ->
       let extract = create d u i' a in
       let mrel = ssa #(secret d u i') in
       let () =
-        MR.m_recall k;
+        recall k;
         let h = get() in
-        assume (MR.m_sel h k == None); // TODO framing of call to create
+        assume (sel h k == None); // TODO framing of call to create
         assume (mrel None (Some extract)); // TODO Fix the monotonic relation
-        MR.m_write k (Some extract) in
+        k := Some extract in
       extract
   else
     let k = psk_real p in
